src/Pipit.Exp.Base.fst
@@ -1,80 +1,156 @@
 module Pipit.Exp.Base
+module C = Pipit.Context
 
-type prim2 =
-  | AndB | OrB | ImpliesB
-  | EqZ
-  | AddZ | SubZ | LeZ // | ...
+(* TODO: restrict "properties" to booleans for now to avoid universe stuff *)
+type xprop = bool
 
-let value  = int
-let var    = nat
-
-let bool_of_value (v: value): bool = v <> 0
-let value_of_bool (b: bool): value = if b then 1 else 0
-
-let eval_prim2 (p: prim2) (v1 : value) (v2: value): value =
-  match p with
-  // XXX: krml does not like to translate short-circuiting (&&) and (||) to C
-  | AndB     -> if bool_of_value v1 then v2 else 0  // value_of_bool (bool_of_value v1 && bool_of_value v2)
-  | OrB      -> if bool_of_value v1 then v1 else v2 // value_of_bool (bool_of_value v1 || bool_of_value v2)
-  | ImpliesB -> if bool_of_value v1 then v2 else 1
-  | EqZ      -> value_of_bool (v1 = v2)
-  | AddZ     -> v1 + v2
-  | SubZ     -> v1 - v2
-  | LeZ      -> value_of_bool (v1 <= v2)
-
-type exp =
+noeq
+type exp (c: C.context) 'a =
   // v
-  | XVal   : value -> exp
-  // x
-  | XVar   : var -> exp
+  | XVal   : 'a -> exp c 'a
+  // bound variable (de Bruijn index)
+  | XBVar  : (i: C.index { C.opt_index c i == Some 'a }) -> exp c 'a
+  // free variables
+  | XVar   : (x: C.var { C.opt_var c x == Some 'a }) -> exp c 'a
   // f(e,...)
-  | XPrim2 : prim2 -> exp -> exp -> exp
-  // if p then e else e'
-  | XIte   : exp -> exp -> exp -> exp
-  // pre e
-  | XPre   : exp -> exp
+  | XApp   : exp c ('b -> 'a) -> exp c 'b -> exp c 'a
+  // v fby e
+  | XFby   : 'a -> exp c 'a -> exp c 'a
   // e -> e'
-  | XThen  : exp -> exp -> exp
+  | XThen  : exp c 'a -> exp c 'a -> exp c 'a
   // µx. e[x]
-  | XMu    : exp -> exp
+  | XMu    : exp (C.bind_index1 c 'a) 'a -> exp c 'a
   // let x = e in e[x]
-  | XLet   : exp -> exp -> exp
+  | XLet   : (b: Type) -> exp c b -> exp (C.bind_index1 c b) 'a -> exp c 'a
 
+  // Proof terms
+  // Contracts for hiding implementation:
+  //   (λx. { assumes } body { λr. guarantees })(arg)
+  | XContract:
+           (assumes: exp (C.from_indices ['b]) xprop) ->
+           (guarantees: exp (C.from_indices ['a; 'b]) xprop) ->
+           (body: exp (C.from_indices ['b]) 'a) ->
+           (arg: exp c 'b) ->
+           exp c 'a
+  // check "" e in e
+  | XCheck : string -> exp c xprop -> exp c 'a -> exp c 'a
 
-let rec wf (e: exp) (n: var): prop =
-match e with
-| XVal _ -> True
-| XVar x -> (x < n) == true
-| XPrim2 _ e1 e2 -> wf e1 n /\ wf e2 n
-| XIte ep et ef -> wf ep n /\ wf et n /\ wf ef n
-| XPre e1 -> wf e1 n
-| XThen e1 e2 -> wf e1 n /\ wf e2 n
-| XMu e1 -> wf e1 (n + 1)
-| XLet e1 e2 -> wf e1 n /\ wf e2 (n + 1)
+let exp' (c: C.closed) 'a = exp c 'a
 
-(* Properties *)
-let rec wf_weaken (e: exp) (n: var) (n': var { n <= n' }):
-  Lemma (requires wf e n)
-        (ensures wf e n') =
+let rec open1' (#c: C.context) (e: exp c 'a) (x: C.var { C.fresh c x }) (n: C.index { C.has_index c n }): Tot (exp (C.open1' c x n) 'a) (decreases e) =
   match e with
-  | XVal _ -> ()
-  | XVar x' -> ()
-  | XPrim2 _ e1 e2 ->
-    wf_weaken e1 n n';
-    wf_weaken e2 n n'
-  | XIte ep e1 e2 ->
-    wf_weaken ep n n';
-    wf_weaken e1 n n';
-    wf_weaken e2 n n'
-  | XPre e1 -> wf_weaken e1 n n'
-  | XThen e1 e2 ->
-    wf_weaken e1 n n';
-    wf_weaken e2 n n'
+  | XVal v -> XVal v
+  | XBVar i ->
+    if i = n
+    then
+      (C.open_contains_opt_var_lemma c x n;
+      XVar x)
+    else
+      (C.open_preserves_opt_index_lemma c x n i;
+      XBVar (C.index_drop i n 1))
+  | XVar x' ->
+    C.open_preserves_opt_var_lemma c x n x';
+    XVar x'
+  | XApp f e -> XApp (open1' f x n) (open1' e x n)
+  | XFby v e -> XFby v (open1' e x n)
+  | XThen e1 e2 -> XThen (open1' e1 x n) (open1' e2 x n)
+  | XMu e -> XMu (open1' e x (n + 1))
+  | XLet b e1 e2 ->
+    let e1' = open1' e1 x n in
+    let e2' = open1' e2 x (n + 1) in
+    XLet b e1' e2'
+  | XContract a g b arg  ->
+    XContract a g b (open1' arg x n)
+  | XCheck name e1 e2 -> XCheck name (open1' e1 x n) (open1' e2 x n)
+
+let rec close1' (#c: C.context) (e: exp c 'a) (x: C.var { C.has_var c x }) (n: C.index { n <= List.Tot.length c.bound }): Tot (exp (C.close1' c x n) 'a) (decreases e) =
+  match e with
+  | XVal v -> XVal v
+  | XBVar i ->
+    C.close_preserves_opt_index_lemma c x n i;
+    XBVar (C.index_lift i n 1)
+  | XVar x' ->
+    if x = x'
+    then
+      (C.close_opt_var_contains_lemma c x n;
+      XBVar n)
+    else
+      (C.close_preserves_opt_var_lemma c x n x';
+      XVar x')
+  | XApp f e -> XApp (close1' f x n) (close1' e x n)
+  | XFby v e -> XFby v (close1' e x n)
+  | XThen e1 e2 -> XThen (close1' e1 x n) (close1' e2 x n)
+  | XMu e -> XMu (close1' e x (n + 1))
+  | XLet b e1 e2 -> XLet b (close1' e1 x n) (close1' e2 x (n + 1))
+  | XContract a g b arg -> XContract a g b (close1' arg x n)
+  | XCheck name e1 e2 -> XCheck name (close1' e1 x n) (close1' e2 x n)
+
+let open1 (e: exp 'c 'a { C.has_index 'c 0 }) x = open1' e x 0
+let close1 (e: exp 'c 'a) x = close1' e x 0
+
+let rec lift1' (#c: C.context) (e: exp c 'a) (n: C.index { n <= List.Tot.length c.bound }) (t: Type): Tot (exp (C.bind_index1' c n t) 'a) (decreases e) =
+  match e with
+  | XVal v -> XVal v
+  | XBVar i ->
+    C.bind_index_preserves_opt_index_lemma c n i t;
+    XBVar (C.index_lift i n 1)
+  | XVar x' ->
+    XVar x'
+  | XApp f e -> XApp (lift1' f n t) (lift1' e n t)
+  | XFby v e -> XFby v (lift1' e n t)
+  | XThen e1 e2 -> XThen (lift1' e1 n t) (lift1' e2 n t)
   | XMu e1 ->
-    wf_weaken e1 (n + 1) (n' + 1)
-  | XLet e1 e2 ->
-    wf_weaken e1 n n';
-    wf_weaken e2 (n + 1) (n' + 1)
+    let e1': exp (C.bind_index1' (C.bind_index1 c 'a) (n + 1) t) 'a = lift1' e1 (n + 1) t in
+    let e1'': exp (C.bind_index1 (C.bind_index1' c n t) 'a) 'a = e1' in
+    XMu e1''
+  | XLet b e1 e2 -> XLet b (lift1' e1 n t) (lift1' e2 (n + 1) t)
+  | XContract a g b arg ->
+    XContract a g b (lift1' arg n t)
+  | XCheck name e1 e2 -> XCheck name (lift1' e1 n t) (lift1' e2 n t)
 
+let lift1 (#c: C.context) (e: exp c 'a) (t: Type): exp (C.bind_index1 c t) 'a =
+  lift1' e 0 t
 
-let xpre_init: value = 0
+let rec subst_index1' (#c: C.context) (e: exp c 'a) (i: C.index { C.has_index c i }) (payload: exp (C.drop_index1 c i) (C.get_index c i)): Tot (exp (C.drop_index1 c i) 'a) (decreases e) =
+  match e with
+  | XVal v -> XVal v
+  | XBVar i' ->
+    if i' = i
+    then payload
+    else
+      (C.drop_index_preserves_opt_index_lemma c i i';
+      XBVar (C.index_drop i' i 1))
+  | XVar x' -> XVar x'
+  | XApp f e -> XApp (subst_index1' f i payload) (subst_index1' e i payload)
+  | XFby v e -> XFby v (subst_index1' e i payload)
+  | XThen e1 e2 -> XThen (subst_index1' e1 i payload) (subst_index1' e2 i payload)
+  | XMu e1 ->
+    let e1': exp (C.drop_index1 (C.bind_index1 c 'a) (i + 1)) 'a = subst_index1' e1 (i + 1) (lift1 payload 'a) in
+    let e1'': exp (C.bind_index1 (C.drop_index1 c i) 'a) 'a = e1' in
+    XMu e1''
+  | XLet b e1 e2 -> XLet b (subst_index1' e1 i payload) (subst_index1' e2 (i + 1) (lift1 payload b))
+  | XContract a g b arg ->
+    XContract a g b (subst_index1' arg i payload)
+  | XCheck name e1 e2 -> XCheck name (subst_index1' e1 i payload) (subst_index1' e2 i payload)
+
+let subst_index1 (#c: C.context { C.has_index c 0 }) (e: exp c 'a) (payload: exp (C.drop_index1 c 0) (C.get_index c 0)): Tot (exp (C.drop_index1 c 0) 'a) (decreases e) =
+  subst_index1' e 0 payload
+
+let rec weaken_closed (#c c': C.closed) (e: exp c 'a): Tot (exp (C.append_closed c c') 'a) (decreases e) =
+  match e with
+  | XVal v -> XVal v
+  | XBVar i' ->
+    C.append_preserves_opt_index_lemma c c' i';
+    XBVar i'
+  | XVar x' -> XVar x'
+  | XApp f e -> XApp (weaken_closed c' f) (weaken_closed c' e)
+  | XFby v e -> XFby v (weaken_closed c' e)
+  | XThen e1 e2 -> XThen (weaken_closed c' e1) (weaken_closed c' e2)
+  | XMu e1 ->
+    let e1': exp (C.append_closed (C.bind_index1 c 'a) c') 'a = weaken_closed c' e1 in
+    let e1'': exp (C.bind_index1 (C.append_closed c c') 'a) 'a = e1' in
+    XMu e1''
+  | XLet b e1 e2 -> XLet b (weaken_closed c' e1) (weaken_closed c' e2)
+  | XContract a g b arg ->
+    XContract a g b (weaken_closed c' arg)
+  | XCheck name e1 e2 -> XCheck name (weaken_closed c' e1) (weaken_closed c' e2)
