src/Pipit.Exp.Causality.fst
@@ -1,3 +1,4 @@
+(*TODO update to typed exprs*)
 module Pipit.Exp.Causality
 
 open Pipit.Exp.Base
